hnorm now supports scheduler macros

scheduler/SchHeader.v
@@ -1,6 +1,6 @@
-Require Import CRIS.
+Require Export Common.
+Require Export SMod HMod PMod.
 Require Import ImpPrelude.
-Require Import wsim.
 
 Module SchName.
   Definition _spawn := "Sch._spawn".
@@ -16,14 +16,6 @@ Section FSpec.
 
   Variable univ: positive.
   Variable StbFun: string → option fspec.
-
-  (* fspec wrapping functions - TODO: move them to a proper file *)
-  (* Definition wfspec_inv (fsp : fspec) : fspec :=
-    mk_fspec (meta := (fsp).(meta))
-      (fun tid x varg arg =>
-        (∃ n, wsats univ n ⊤) ∗ fsp.(precond) tid x varg arg)%I
-      (fun tid x vret ret =>
-        (∃ n, wsats univ n ⊤) ∗ fsp.(postcond) tid x vret ret)%I. *)
 
   Definition sfunN {X Y} `{coreE -< E} `{callE -< E} `{pgE -< E}
       (body : X -> itree E Y) : SAny.t -> itree E SAny.t :=
@@ -54,18 +46,17 @@ Section FSpec.
     end.
 End FSpec.
 
-Module Sch. Section MACRO.
+Module Sch. Section Sch.
   Import Events.
 
-  Context {E: Type → Type}.
+  Context {E : Type → Type}.
   Context `{coreE -< E, callE -< E}.
 
   Definition spawn : (string * SAny.t) → itree E nat :=
     Seal.sealing "Sch"
       (λ fnarg,
         'tid: nat <- ccallU SchName.spawn fnarg;;
-        Ret tid)
-  .
+        Ret tid).
 
   Definition yield : itree E unit :=
     Seal.sealing "Sch"
@@ -76,30 +67,129 @@ Module Sch. Section MACRO.
         else
           '():_ <- ccallU SchName.yield tt;;
           Ret (inl tt: () + ())
-      )) tt)
-  .
+      )) tt).
 
   Definition terminate : itree E unit :=
     Seal.sealing "Sch"
       (ITree.iter ((fun (_: unit) =>
         '():_ <- ccallU SchName.yield tt;;
         Ret (inl tt: () + ())
-      )) tt)
-  .
+      )) tt).
 
-  Definition join (R: Type): nat → itree E R :=
+  Definition join (R : Type) : nat → itree E R :=
     Seal.sealing "Sch"
       (λ tid,
         'ora: option SAny.t <- ccallU SchName.join tid;;
         ra <- ora?;;
         rv <- (ra↓↓)?;;
-        Ret rv)
-  .
+        Ret rv).
 
-End MACRO. End Sch.
+  Definition spawnK {R} (fnarg : string * SAny.t) (k : nat → itree E R) : itree E R :=
+    'tid : nat <- ccallU SchName.spawn fnarg;;
+    k tid.
+
+  Definition yieldK {R} (k : itree E R) : itree E R :=
+    yield;;; k.
+
+  Definition joinK {R R'} (tid : nat) (k : R → itree E R') : itree E R' :=
+    'r : R <- join R tid;;
+    k r.
+
+  Lemma spawn_spawnK fnargs : spawn fnargs = spawnK fnargs (λ x, Ret x).
+  Proof. rewrite /spawnK /spawn; unseal "Sch". ss. Qed.
+
+  Lemma yield_yieldK : yield = yieldK (Ret tt).
+  Proof.
+    rewrite /yieldK. rewrite {1} (bind_ret_r_rev yield). f_equal; ss.
+    extensionalities x; destruct x; ss.
+  Qed.
+
+  Lemma join_joinK R tid : join R tid = joinK tid (λ x, Ret x).
+  Proof.
+    rewrite /joinK /join; unseal "Sch". grind. rewrite {1}(bind_ret_r_rev (unwrapU _)).
+    f_equal. extensionalities y; grind.
+  Qed.
+End Sch.
+Section Sch.
+  Context {Σ : GRA}.
+
+  Definition yieldK_S {R} ginv stb (k : itree hmodE R) : itree hmodE R :=
+    interp_smod ginv stb yield;;; k.
+
+  Definition yieldK_S_SB {R} ginv stb scopes (k : itree hmodE R) : itree hmodE R :=
+    HMod.sandbox scopes (interp_smod ginv stb yield);;; k.
+
+  Lemma yieldK_bind {R R'} (k1 : itree hmodE R) (k2 : R → itree hmodE R') :
+    yieldK k1 >>= k2 = yieldK (k1 >>= k2).
+  Proof. rewrite /yieldK; grind. Qed.
+
+  Lemma yieldK_S_SB_yield {R} ginv stb scopes (k : itree hmodE R) :
+    yieldK_S_SB ginv stb scopes k = HMod.sandbox scopes (interp_smod ginv stb yield);;; k.
+  Proof. ss. Qed.
+
+  Lemma yieldK_interp_smod {R} ginv stb (k : itree hmodE R) :
+    interp_smod ginv stb (yieldK k) = yieldK_S ginv stb (interp_smod ginv stb k).
+  Proof. rewrite /yieldK /yieldK_S SModRed.interp_bind; ss. Qed.
+
+  Lemma yieldK_S_transl {R} scopes ginv stb (k : itree hmodE R) :
+    HMod.sandbox scopes (yieldK_S ginv stb k)
+    = yieldK_S_SB ginv stb scopes (HMod.sandbox scopes k).
+  Proof. rewrite /yieldK_S /yieldK_S_SB HModSB.transl_bind //. Qed.
+
+  Definition spawnK_S {R} ginv stb fnargs (k : nat → itree hmodE R) : itree hmodE R :=
+    x <- interp_smod ginv stb (spawn fnargs);; k x.
+
+  Definition spawnK_S_SB {R} ginv stb scopes fnargs (k : nat → itree hmodE R) : itree hmodE R :=
+    x <- HMod.sandbox scopes (interp_smod ginv stb (spawn fnargs));; k x.
+
+  Lemma spawnK_bind {R R'}
+      (fnarg : string * SAny.t) (k1 : nat → itree hmodE R) (k2 : R → itree hmodE R') :
+    spawnK fnarg k1 >>= k2 = spawnK fnarg (λ n, (k1 n) >>= k2).
+  Proof. rewrite /spawnK. grind. Qed.
+
+  Lemma spawnK_S_SB_spawn {R} ginv stb scopes fnarg (k : nat → itree hmodE R) :
+    spawnK_S_SB ginv stb scopes fnarg k
+    = HMod.sandbox scopes (interp_smod ginv stb (spawn fnarg)) >>= k.
+  Proof. ss. Qed.
+
+  Lemma spawnK_interp_smod {R} ginv stb fnargs (k : nat → itree hmodE R) :
+    interp_smod ginv stb (spawnK fnargs k)
+    = spawnK_S ginv stb fnargs (λ x, interp_smod ginv stb (k x)).
+  Proof. rewrite /spawnK_S /spawnK /spawn SModRed.interp_bind; unseal "Sch". grind. Qed.
+
+  Lemma spawnK_S_transl {R} ginv stb scopes fnargs (k : nat → itree hmodE R) :
+    HMod.sandbox scopes (spawnK_S ginv stb fnargs k)
+    = spawnK_S_SB ginv stb scopes fnargs (λ x, HMod.sandbox scopes (k x)).
+  Proof. rewrite /spawnK_S_SB /spawnK_S /spawn; unseal "Sch"; rewrite HModSB.transl_bind; ss. Qed.
+
+  Definition joinK_S {R R'} ginv stb tid (k : R' → itree hmodE R) : itree hmodE R :=
+    x <- interp_smod ginv stb (join R' tid);; k x.
+
+  Definition joinK_S_SB {R R'} ginv stb scopes tid (k : R' → itree hmodE R) : itree hmodE R :=
+    x <- HMod.sandbox scopes (interp_smod ginv stb (join R' tid));; k x.
+
+  Lemma joinK_bind {R R1 R2} (tid : nat) (k1 : R → itree hmodE R1) (k2 : R1 → itree hmodE R2) :
+    joinK tid k1 >>= k2 = joinK tid (λ x, k1 x >>= k2).
+  Proof. rewrite /joinK; grind. Qed.
+
+  Lemma joinK_S_SB_join {R R'} ginv stb scopes tid (k : R' → itree hmodE R) :
+    joinK_S_SB ginv stb scopes tid k
+    = HMod.sandbox scopes (interp_smod ginv stb (join R' tid)) >>= k.
+  Proof. ss. Qed.
+
+  Lemma joinK_interp_smod {R R'} ginv stb tid (k : R' → itree hmodE R) :
+    interp_smod ginv stb (joinK tid k)
+    = joinK_S ginv stb tid (λ x, interp_smod ginv stb (k x)).
+  Proof. rewrite /joinK_S /joinK /join SModRed.interp_bind; unseal "Sch". grind. Qed.
+
+  Lemma joinK_S_transl {R R'} ginv stb scopes tid (k : R' → itree hmodE R) :
+    HMod.sandbox scopes (joinK_S ginv stb tid k)
+    = joinK_S_SB ginv stb scopes tid (λ x, HMod.sandbox scopes (k x)).
+  Proof. rewrite /joinK_S_SB /joinK_S /join; unseal "Sch"; rewrite HModSB.transl_bind; ss. Qed.
+End Sch. End Sch.
 
 Notation "x <- t1 ||; t2" := (ITree.bind t1 (fun x => (Sch.yield ;;; t2)))
-  (at level 62, t1 at next level, right associativity) : itree_scope.
+  ( at level 62, t1 at next level, right associativity) : itree_scope.
 Notation "t1 ||;; t2" := (ITree.bind t1 (fun _ => (Sch.yield ;;;t2)))
   (at level 62, right associativity) : itree_scope.
 Notation "' p : T <- t1 ||; t2" :=
