examples/ring/RingA.v
@@ -79,6 +79,6 @@ Module RingA. Section RingA.
   Definition InitCond : iProp Σ :=
     ([∗ list] i↦_ ∈ (replicate max_size 0%Z), CellAS.pending i)%I.
 
-  Definition t Spc := Seal.sealing CRIS (SMod.to_hmod ginv_emp Spc Mod).
+  Definition t Spc := Seal.sealing CRIS (SMod.to_hmod emp Spc Mod).
 
 End RingA. End RingA.
